binomial development

proof/misc/ideal.ec
@@ -12,16 +12,45 @@
 (* Requirements           *)
 (**************************)
 
-require import AllCore List Ring.
+require import AllCore List Ring StdRing.
 require (*--*) Bigalg.
 
 clone include Ring.ComRing.
 
-clone import Bigalg.BigComRing with type t <- t.
+clone import Bigalg.BigComRing with
+  type t <- t,
+  pred CR.unit   <- Top.unit,
+    op CR.zeror  <- Top.zeror,
+    op CR.oner   <- Top.oner,
+    op CR.( + )  <- Top.( + ),
+    op CR.([-])  <- Top.([-]),
+    op CR.( * )  <- Top.( * ),
+    op CR.invr   <- Top.invr,
+    op CR.intmul <- Top.intmul,
+    op CR.ofint  <- Top.ofint,
+    op CR.exp    <- Top.exp
+
+    proof CR.*
+
+    remove abbrev CR.(-)
+    remove abbrev CR.(/).
+
+realize CR.addrA      by apply Top.addrA    .
+realize CR.addrC      by apply Top.addrC    .  
+realize CR.add0r      by apply Top.add0r    . 
+realize CR.addNr      by apply Top.addNr    . 
+realize CR.oner_neq0  by apply Top.oner_neq0. 
+realize CR.mulrA      by apply Top.mulrA    . 
+realize CR.mulrC      by apply Top.mulrC    . 
+realize CR.mul1r      by apply Top.mul1r    . 
+realize CR.mulrDl     by apply Top.mulrDl   . 
+realize CR.mulVr      by apply Top.mulVr    . 
+realize CR.unitP      by apply Top.unitP    . 
+realize CR.unitout    by apply Top.unitout  . 
 
 instance ring with t
-  op rzero = zeror
-  op rone  = oner
+  op rzero = Top.zeror
+  op rone  = Top.oner
   op add   = Top.( + )
   op opp   = Top.([-])
   op mul   = Top.( * )
@@ -39,7 +68,45 @@ instance ring with t
   proof expr0     by apply/expr0
   proof exprS     by apply/exprS.
 
+(* -------------------------------------------------------------------- *)
+hint simplify expr0, expr1.
 
+(* There is a Binomial.ec file in the std library that seems incomplete *)
+op c : int -> int -> int.
+
+lemma cn0 n : c n 0 = 1 by admit.
+lemma cnn n : c n n = 1 by admit.
+
+lemma ge0_c n m : 0 <= c n m by admit.
+
+lemma PascalTriangle n k :
+  0 <= n => 0 <= k < n => c n k + c n (k+1) = c (n+1) (k+1).
+proof. admitted.
+
+lemma mulrDz (x : t) (n m : int) : intmul x (n + m) = intmul x n + intmul x m.
+proof. admitted.
+
+lemma binomial x y n : 0 <= n => exp (x + y) n =
+  BAdd.bigi predT (fun i => intmul (exp x i * exp y (n - i)) (c n i)) 0 (n + 1).
+proof.
+elim: n => [|i ge0_i ih].
++ by rewrite BAdd.big_int1 /= mul1r cn0 mulr1z.
+rewrite exprS // ih /= mulrDl 2!BAdd.mulr_sumr.
+rewrite (BAdd.big_addn 1 _ (-1)) /= (BAdd.big_int_recr (i+1)) 1:/# /=.
+pose s1 := BAdd.bigi _ _ _ _; rewrite cnn mulr1z mulr1 -exprS // addrAC.
+apply: eq_sym; rewrite (BAdd.big_int_recr (i+1)) 1:/# /= cnn mulr1z mulr1.
+congr; apply: eq_sym; rewrite (BAdd.big_int_recl _ 0) //=.
+rewrite cn0 mulr1z mul1r -exprS // addrCA addrC; apply: eq_sym.
+rewrite (BAdd.big_int_recl _ 0) //= cn0 mulr1z mul1r addrC.
+congr; apply: eq_sym; rewrite /s1 => {s1}.
+rewrite !(BAdd.big_addn 1 _ (-1)) /= -BAdd.big_split /=.
+rewrite !BAdd.big_seq &(BAdd.eq_bigr) => /= j /mem_range rg_j.
+rewrite mulrnAr ?ge0_c mulrA -exprS 1:/# /= addrC.
+rewrite mulrnAr ?ge0_c mulrCA -exprS 1:/#.
+rewrite IntID.addrAC IntID.opprB IntID.addrA.
+rewrite -mulrDz; congr; rewrite IntID.addrC.
+by rewrite (PascalTriangle i (j-1)) 1,2:/#.
+qed.
 
 (**************************)
 (* Operators              *)
